%===============================================================================
\section{Interpretación}
%===============================================================================
\begin{frame}{Interpretación}
	\begin{itemize}
		\item $\hat{y}=\hat{\beta_{0}}+\hat\beta_{1}x_{1}+\hat\beta_{2}x_{2}+...+\hat\beta_{k}x_{k}$\\
		Tomando el operador diferencial:
		\item $\Delta\hat{y}=\hat\beta_{1}\Delta x_{1}+\hat\beta_{2}\Delta x_{2}+...+\hat\beta_{k}\Delta x_{k}$ \\
		Así, manteniendo fijos $x_{2},...,x_{k}$, entonces
		\item $\Delta\hat{y}=\hat{\beta_{1}}\Delta x_{1}$\\
		Interpretar
		\bigskip
		\begin{enumerate}
			\item $Ln(y)=\hat\beta_{0}+\hat\beta_{1} Ln(x_{1})$
			\item $Ln(y)=\hat\beta_{0}+\hat\beta_{1} x_{1}$
			\item $y=\hat{\beta_{0}}+\hat\beta_{1} Ln(x_{1})$
		\end{enumerate}
	\end{itemize}
\end{frame}
